

## Exercise Sheet 11

Due: December 04, 2025

Vincent Xigu Liu (25-927-229, TA: Moeto Suzuki)

---

### Exercise 11.2

1)

**Lemma Ex. 11.2.1:**

Let  $\parallel$  denote the concatenation operation. Let  $+$  denote the arithmetic sum operation. Then we have

$$\forall x \in \mathcal{C} : \left( \exists a, b \in \bigcup_{i \in \mathbb{N}^*} F^i : a \parallel b = x \right) \rightarrow \text{hw}(a) + \text{hw}(b) = \text{hw}(x)$$

**Proof.**

Let  $x = (x_1, x_2, \dots, x_n)$  for all sequences  $x$ . We define the indicator function:

$$k_i(x) = \begin{cases} 1 & \text{if } x_i \neq 0 \\ 0 & \text{otherwise} \end{cases}$$

Then, we have for the Hamming weight of  $x$  the following splitting:

$$k_i(x) = \begin{cases} k_i(a) & \text{if } 1 \leq i \leq |a| \\ k_{i-|a|}(b) & \text{if } |a| + 1 \leq i \leq n \end{cases}$$

which gives

$$\text{hw}(x) = \sum_{i=1}^n k_i(x) = \sum_{i=1}^{|a|} k_i(a) + \sum_{i=|a|+1}^n k_{i-|a|}(b) = \text{hw}(a) + \text{hw}(b)$$

□

**Lemma Ex. 11.2.2:**

Let  $u$  be a sequence over  $F^n$ ,  $n \in \mathbb{N}^*$ . Then,

$$\text{hw}(u) = \text{hw}(-u)$$

**Proof.** Let  $u = (u_1, u_2, \dots, u_n)$ . Then, we have

$$-u = (-u_1, -u_2, \dots, -u_n)$$

and according to the definition of Hamming weight, we have

$$\text{hw}(u) = \sum_{i \in [n]} \begin{cases} 0 & \text{if } u_i = 0 \\ 1 & \text{otherwise} \end{cases}$$

and

$$\text{hw}(-u) = \sum_{i \in [n]} \begin{cases} 0 & \text{if } -u_i = 0 \\ 1 & \text{otherwise} \end{cases}$$

However, according to the properties of a field, we have

$$u_i = 0 \Leftrightarrow -u_i = 0$$

so in all positions  $i \in [n]$ , the contribution to the Hamming weight from  $u_i$  and  $-u_i$  are the same.  $\square$

According to Lemma Ex. 11.2.1, as

$$x = (x_1, x_2, \dots, x_n) = x_1 \parallel x_2 \parallel \dots \parallel x_n$$

we have

$$\begin{aligned} \text{hw}(x) &= \sum_{i \in [n]} \text{hw}(x_i) \wedge \text{hw}(y) = \sum_{i \in [n]} \text{hw}(y_i) \\ \Rightarrow \text{hw}(x) + \text{hw}(y) &= \sum_{i \in [n]} \text{hw}(x_i) + \sum_{i \in [n]} \text{hw}(y_i) = \sum_{i \in [n]} \text{hw}(x_i) + \text{hw}(y_i) \end{aligned}$$

analogously, we have

$$\text{hw}(x + y) = \sum_{i \in [n]} \text{hw}(x_i + y_i)$$

We notice that

$$\begin{aligned} x_i = 0 \wedge y_i = 0 &\Rightarrow x_i + y_i = 0 \Rightarrow \text{hw}(x_i + y_i) = 0 \wedge \text{hw}(x_i) + \text{hw}(y_i) = 0 + 0 = 0 \\ x_i = 0 \wedge y_i \neq 0 &\Rightarrow x_i + y_i \neq 0 \Rightarrow \text{hw}(x_i + y_i) = 1 \wedge \text{hw}(x_i) + \text{hw}(y_i) = 0 + 1 = 1 \\ x_i \neq 0 \wedge y_i = 0 &\Rightarrow x_i + y_i \neq 0 \Rightarrow \text{hw}(x_i + y_i) = 1 \wedge \text{hw}(x_i) + \text{hw}(y_i) = 1 + 0 = 1 \\ x_i \neq 0 \wedge y_i \neq 0 &\Rightarrow x_i + y_i \neq 0 \Rightarrow \text{hw}(x_i + y_i) = 1 \wedge \text{hw}(x_i) + \text{hw}(y_i) = 1 + 1 = 2 \end{aligned}$$

as in all cases,

$$\text{hw}(x_i + y_i) \leq \text{hw}(x_i) + \text{hw}(y_i)$$

we have

$$\text{hw}(x + y) = \sum_{i \in [n]} \text{hw}(x_i + y_i) \leq \sum_{i \in [n]} \text{hw}(x_i) + \text{hw}(y_i) = \text{hw}(x) + \text{hw}(y)$$

with which our claim is proven.

2)

1.  $d_{\min}(\mathcal{C}) \leq \min_{c \in \mathcal{C} - \{0^n\}} \text{hw}(c)$ :

suppose that there is a  $c \in \mathcal{C} - \{0^n\}$  with  $\text{hw}(c) < d_{\min}(\mathcal{C})$ . Then, the Hamming distance between  $0^n$  and  $c$  is exactly  $\text{hw}(c)$ , so  $d(0^n, c) < d_{\min}(\mathcal{C})$  which is a contradiction, so the opposite is proven.

2.  $d_{\min}(\mathcal{C}) \geq \min_{c \in \mathcal{C} - \{0^n\}} \text{hw}(c)$ :

suppose that there is  $a, b \in \mathcal{C}$  with  $d(a, b) < \min_{c \in \mathcal{C} - \{0^n\}}$ . Then, let  $a_n = a + (-a) = 0$ ,  $b_n = b + (-a)$ . The hamming distance remains the same because for all positions  $i \in [n]$ , if  $a_i = b_i$  then  $a_i + (-a_i) = b_i + (-a_i)$ , else  $a_i \neq b_i$  implies  $a_i + (-a_i) \neq b_i + (-a_i)$ . So we have  $d(a_n, b_n) = d(a, b) < \min_{c \in \mathcal{C} - \{0^n\}}$ . However,  $d(a_n, b_n) = \text{hw}(b_n)$  and  $b_n \in \mathcal{C} - \{0^n\}$ , which is a contradiction. So the opposite is proven.

Combining 1. and 2), we have

$$d_{\min}(\mathcal{C}) = \min_{c \in \mathcal{C} - \{0^n\}} \text{hw}(c)$$

3)

According to 2), we have

$$\begin{aligned} d_{\min}(\mathcal{D}) &= \min_{d \in \mathcal{D} - \{0^{2n}\}} \text{hw}(d) \\ \wedge d_{\min}(U) &= \min_{u \in \mathcal{U} - \{0^n\}} \text{hw}(u) \\ \wedge d_{\min}(V) &= \min_{v \in \mathcal{V} - \{0^n\}} \text{hw}(v) \end{aligned}$$

so it is sufficient to prove that

$$\Rightarrow \min_{d \in \mathcal{D} - \{0^{2n}\}} \text{hw}(d) = \min \left( 2 * \min_{u \in \mathcal{U} - \{0^n\}} \text{hw}(u), \min_{v \in \mathcal{V} - \{0^n\}} \text{hw}(v) \right)$$

we prove in both directions:

$$1. \min_{d \in \mathcal{D} - \{0^{2n}\}} \text{hw}(d) \leq \min \left( 2 * \min_{u \in \mathcal{U} - \{0^n\}} \text{hw}(u), \min_{v \in \mathcal{V} - \{0^n\}} \text{hw}(v) \right):$$

$$\text{Case 1: } 2 * \min_{u \in \mathcal{U} - \{0^n\}} \text{hw}(u) \leq \min_{v \in \mathcal{V} - \{0^n\}} \text{hw}(v)$$

In this case, let  $v = 0^n$ . Then, we have  $u \| u \in \mathcal{D}$  and  $\text{hw}(u \| u) = 2 * \text{hw}(u)$ . Hence, we have

$$\begin{aligned} \min_{d \in \mathcal{D} - \{0^{2n}\}} \text{hw}(d) &\leq \text{hw}(u \| u) = 2 * \text{hw}(u) = 2 * \min_{u \in \mathcal{U} - \{0^n\}} \text{hw}(u) \\ &= \min \left( 2 * \min_{u \in \mathcal{U} - \{0^n\}} \text{hw}(u), \min_{v \in \mathcal{V} - \{0^n\}} \text{hw}(v) \right) \end{aligned}$$

$$\text{Case 2: } 2 * \min_{u \in \mathcal{U} - \{0^n\}} \text{hw}(u) > \min_{v \in \mathcal{V} - \{0^n\}} \text{hw}(v)$$

In this case, let  $u = 0^n$ . Then, we have  $0^n \| v \in \mathcal{D}$  and  $\text{hw}(0^n \| v) = \text{hw}(v)$ . Hence, we have

$$\begin{aligned} \min_{d \in \mathcal{D} - \{0^{2n}\}} \text{hw}(d) &\leq \text{hw}(0^n \| v) = \text{hw}(v) = \min_{v \in \mathcal{V} - \{0^n\}} \text{hw}(v) \\ &= \min \left( 2 * \min_{u \in \mathcal{U} - \{0^n\}} \text{hw}(u), \min_{v \in \mathcal{V} - \{0^n\}} \text{hw}(v) \right) \end{aligned}$$

As the case distinction is complete, the claim is proven.

$$2. \min_{d \in \mathcal{D} - \{0^{2n}\}} \text{hw}(d) \geq \min \left( 2 * \min_{u \in \mathcal{U} - \{0^n\}} \text{hw}(u), \min_{v \in \mathcal{V} - \{0^n\}} \text{hw}(v) \right):$$

Suppose that there is a  $d \in \mathcal{D} - \{0^{2n}\}$  with

$$\text{hw}(d) < \min \left( 2 * \min_{u \in \mathcal{U} - \{0^n\}} \text{hw}(u), \min_{v \in \mathcal{V} - \{0^n\}} \text{hw}(v) \right)$$

Let  $d = u \parallel (u + v)$  with  $u \in \mathcal{U}, v \in \mathcal{V}$ .

**Case 1:**  $v = 0^n$

In this case,  $u \neq 0^n$  because otherwise  $d = 0^{2n}$ . So we have

$$\begin{aligned} \text{hw}(d) &= \text{hw}(u \parallel (u + 0^n)) = \text{hw}(u \parallel u) \\ &= 2 * \text{hw}(u) \geq 2 * \min_{u \in \mathcal{U} - \{0^n\}} \text{hw}(u) \geq \min \left( 2 * \min_{u \in \mathcal{U} - \{0^n\}} \text{hw}(u), \min_{v \in \mathcal{V} - \{0^n\}} \text{hw}(v) \right) \end{aligned}$$

which is a contradiction.

**Case 2:**  $v \neq 0^n$

In this case, we have

$$\begin{aligned} \text{hw}(d) &= \text{hw}(u \parallel (u + v)) = \text{hw}(u) + \text{hw}(u + v) \\ &= \text{hw}(-u) + \text{hw}(u + v) \geq \text{hw}(v + u - u) \\ &= \text{hw}(v) \geq \min_{v \in \mathcal{V} - \{0^n\}} \text{hw}(v) \geq \min \left( 2 * \min_{u \in \mathcal{U} - \{0^n\}} \text{hw}(u), \min_{v \in \mathcal{V} - \{0^n\}} \text{hw}(v) \right) \end{aligned}$$

which is a contradiction.

As the case distinction is complete, the claim is proven.

As both directions are proven, we have

$$\min_{d \in \mathcal{D} - \{0^{2n}\}} \text{hw}(d) = \min \left( 2 * \min_{u \in \mathcal{U} - \{0^n\}} \text{hw}(u), \min_{v \in \mathcal{V} - \{0^n\}} \text{hw}(v) \right)$$

which is exactly what we wanted to show.